yalla/mgraph_tree.v
@@ -1,0 +1,368 @@
+(* Extension for [mgraph] of the library GraphTheory
+   About Trees
+ *)
+
+From Coq Require Import Bool.
+Set Warnings "-notation-overridden". (* to ignore warnings due to the import of ssreflect *)
+From mathcomp Require Import all_ssreflect zify.
+Set Warnings "notation-overridden".
+From GraphTheory Require Import preliminaries mgraph structures bij setoid_bigop.
+From Yalla Require Import mll_prelim graph_more.
+
+Import EqNotations.
+
+Set Mangle Names.
+Set Mangle Names Light.
+Set Implicit Arguments.
+Unset Strict Implicit.
+Unset Printing Implicit Defensive.
+Set Bullet Behavior "Strict Subproofs".
+
+
+Section Tree.
+Context {Lv Le : Type} {G : graph Lv Le}.
+
+(* Tree = acyclic and connected graph *)
+Definition utree {I : eqType} (f : edge G -> option I) :=
+  uacyclic f /\ uconnected f.
+
+(* In an acyclic graph (where we removed only edges), there is at most one path between two vertices *)
+Lemma uacyclic_unique_path {I : finType} (f : edge G -> option I) :
+  {in ~: f @^-1 None &, injective f} -> uacyclic f -> forall (s t : G) (p q : Supath f s t), p = q.
+Proof.
+  intros F A s t [p P] [q Q]. cbnb.
+  destruct (eq_comparable p q) as [ | Neq]; trivial.
+  exfalso.
+  revert s P q Q Neq. induction p as [ | [ep bp] p IHp] => s P q Q Neq; destruct q as [ | [eq bq] q]; try by [].
+  - revert P. rewrite /supath /= !andb_true_r => /eqP-?. subst t.
+    by specialize (A _ {| upval := _ ; upvalK := Q |}).
+  - revert Q. rewrite /supath /= !andb_true_r => /eqP-?. subst t.
+    by specialize (A _ {| upval := _ ; upvalK := P |}).
+  - assert (Pe : supath f s t ((ep, bp) :: p)) by assumption.
+    assert (Qe : supath f s t ((eq, bq) :: q)) by assumption.
+    revert P. rewrite /supath /= in_cons => /andP[/andP[/andP[/eqP-SP WP] /andP[uP UP]] /norP[/eqP-nP NP]].
+    revert Q. rewrite /supath /= in_cons => /andP[/andP[/andP[/eqP-SQ WQ] /andP[uQ UQ]] /norP[/eqP-nQ NQ]].
+    destruct (eq_comparable ep eq) as [ | Hneq]; [subst eq | ].
+    + assert (bp = bq).
+      { destruct (eq_comparable bp bq) as [ | Hneq]; trivial.
+        contradict SQ. rewrite -SP.
+        destruct bp, bq; try by [].
+        - by apply nesym, (uacyclic_loop A), nesym.
+        - by apply (uacyclic_loop A), nesym. }
+      subst bq.
+      revert Neq => /eqP. cbn. move => /nandP[/nandP[/eqP // | /eqP //] | /eqP-Neq].
+      eapply (IHp (endpoint bp ep) _ q _ Neq). Unshelve. splitb. splitb.
+    + clear Neq IHp.
+      set pq : upath := p ++ upath_rev q.
+      assert (WPQ : uwalk (endpoint bp ep) (endpoint bq eq) pq).
+      { apply (uwalk_cat WP). by rewrite uwalk_rev. }
+      assert (NPQ : None \notin [seq f e.1 | e <- pq]).
+      { rewrite /pq map_cat mem_cat. splitb.
+        by rewrite map_comp upath_rev_fst map_rev in_rev -map_comp. }
+      destruct (uconnected_simpl F WPQ NPQ) as [PQ' HPQ'].
+      assert (Eq : supath f (endpoint bq eq) (endpoint (~~bq) eq) [:: (eq, ~~bq)]).
+      { rewrite /supath !in_cons /= orb_false_r negb_involutive. splitb. by apply /eqP. }
+      set EQ := {| upval := _ ; upvalK := Eq |}.
+      assert (Ep : supath f (endpoint (~~bp) ep) (endpoint bp ep) [:: (ep, bp)]).
+      { rewrite /supath !in_cons /= orb_false_r. splitb. by apply /eqP. }
+      set EP := {| upval := _ ; upvalK := Ep |}.
+      assert (Qep : ep \notin [seq e.1 | e <- q]).
+      { remember (ep \in [seq e.1 | e <- q]) as b eqn:In. symmetry in In.
+        destruct b; trivial.
+        assert (exists b, (ep, b) \in q) as [b In'] by by apply in_map_fst.
+        clear In.
+        apply in_elt_sub in In'.
+        assert (In'' : exists (n : nat), q == take n q ++ (ep, b) :: drop n.+1 q).
+        { destruct In' as [n ?]. exists n. by apply /eqP. }
+        revert In'' => {In'} /sigW[n /eqP-Qeq].
+        rewrite Qeq in Qe.
+        destruct (eq_comparable b bp).
+        - subst b.
+          assert (Hr : (eq, bq) :: take n q ++ (ep, bp) :: drop n.+1 q =
+            ((eq, bq) :: take n q) ++ [:: (ep, bp)] ++ drop n.+1 q).
+          { by rewrite -(cat1s (ep, bp) (drop n.+1 q))
+                       -(cat1s (eq, bq) ((take n q) ++ ([:: (ep, bp)] ++ (drop n.+1 q))))
+                       -(cat1s (eq, bq) (take n q)) -!catA. }
+          rewrite Hr {Hr} in Qe.
+          destruct (supath_subKK Qe) as [L _].
+          assert (Hr : (upath_target s ((eq, bq) :: (take n q))) = s).
+          { transitivity (upath_source t ([:: (ep, bp)] ++ (drop n.+1 q))); last by rewrite /= SP.
+            apply uwalk_sub_middle.
+            by revert Qe => /andP[/andP[-> _] _]. }
+          rewrite Hr {Hr} in L.
+          specialize (A s {| upval := _ ; upvalK := L |}).
+          contradict A. cbnb.
+        - assert (b = ~~bp) by by destruct b, bp.
+          subst b.
+          assert (Hr : (eq, bq) :: take n q ++ (ep, ~~ bp) :: drop n.+1 q =
+            (((eq, bq) :: take n q) ++ [:: (ep, ~~ bp)]) ++ drop n.+1 q).
+          { by rewrite -(cat1s (ep, ~~ bp) (drop n.+1 q))
+                       -(cat1s (eq, bq) ((take n q) ++ ([:: (ep, ~~ bp)] ++ (drop n.+1 q))))
+                       -(cat1s (eq, bq) (take n q)) -!catA. }
+          rewrite Hr {Hr} in Qe.
+          destruct (supath_subKK Qe) as [L _].
+          rewrite /= map_cat /= last_cat /= SP in L.
+          specialize (A s {| upval := _ ; upvalK := L |}).
+          contradict A. cbnb. }
+      assert (Peq : eq \notin [seq e.1 | e <- p]).
+      (* TODO same as Qep above: possible to do the 2 in 1 with a wlog/forall? *)
+      { remember (eq \in [seq e.1 | e <- p]) as b eqn:In. symmetry in In.
+        destruct b; trivial.
+        assert (exists b, (eq, b) \in p) as [b In'] by by apply in_map_fst.
+        clear In.
+        apply in_elt_sub in In'.
+        assert (In'' : exists (n : nat), p == take n p ++ (eq, b) :: drop n.+1 p).
+        { destruct In' as [n ?]. exists n. by apply /eqP. }
+        revert In'' => {In'} /sigW[n /eqP-Peq].
+        rewrite Peq in Pe.
+        destruct (eq_comparable b bq).
+        - subst b.
+          assert (Hr : (ep, bp) :: take n p ++ (eq, bq) :: drop n.+1 p =
+            ((ep, bp) :: take n p) ++ [:: (eq, bq)] ++ drop n.+1 p).
+          { by rewrite -(cat1s (eq, bq) (drop n.+1 p))
+                       -(cat1s (ep, bp) ((take n p) ++ ([:: (eq, bq)] ++ (drop n.+1 p))))
+                       -(cat1s (ep, bp) (take n p)) -!catA. }
+          rewrite Hr {Hr} in Pe.
+          destruct (supath_subKK Pe) as [L _].
+          assert (Hr : (upath_target s ((ep, bp) :: (take n p))) = s).
+          { transitivity (upath_source t ([:: (eq, bq)] ++ (drop n.+1 p))); last by rewrite /= SQ.
+            apply uwalk_sub_middle.
+            by revert Pe => /andP[/andP[-> _] _]. }
+          rewrite Hr {Hr} in L.
+          specialize (A s {| upval := _ ; upvalK := L |}).
+          contradict A. cbnb.
+        - assert (b = ~~bq) by by destruct b, bq.
+          subst b.
+          assert (Hr : (ep, bp) :: take n p ++ (eq, ~~ bq) :: drop n.+1 p =
+            (((ep, bp) :: take n p) ++ [:: (eq, ~~ bq)]) ++ drop n.+1 p).
+          { by rewrite -(cat1s (eq, ~~ bq) (drop n.+1 p))
+                       -(cat1s (ep, bp) ((take n p) ++ ([:: (eq, ~~ bq)] ++ (drop n.+1 p))))
+                       -(cat1s (ep, bp) (take n p)) -!catA. }
+          rewrite Hr {Hr} in Pe.
+          destruct (supath_subKK Pe) as [L _].
+          rewrite /= map_cat /= last_cat /= SQ in L.
+          specialize (A s {| upval := _ ; upvalK := L |}).
+          contradict A. cbnb. }
+      assert (DQ : upath_disjoint f PQ' EQ).
+      { rewrite /upath_disjoint disjoint_sym disjoint_has /= orb_false_r.
+        apply /mapP. move => [[k b] K /= KEQ].
+        specialize (HPQ' _ K). clear K.
+        assert (eq = k).
+        { apply F; trivial.
+          - rewrite !in_set. apply /eqP. by apply nesym.
+          - rewrite !in_set. apply /eqP => FK.
+            contradict NPQ. apply /negP/negPn.
+            rewrite -FK.
+            replace k with ((k, b).1) by trivial.
+            by apply (map_f (fun e => f e.1)). }
+        subst k. clear KEQ.
+        revert HPQ'. rewrite /pq mem_cat upath_rev_in => /orP[In | In].
+        - contradict Peq. apply /negP/negPn.
+          replace eq with ((eq, b).1) by trivial.
+          by apply map_f.
+        - contradict uQ. apply /negP/negPn.
+          replace eq with ((eq, ~~b).1) by trivial.
+          by apply (map_f (fun e => f e.1)). }
+      set PQ'Q := supath_cat DQ.
+      assert (DP : upath_disjoint f EP PQ'Q).
+      { rewrite /upath_disjoint disjoint_has /= map_cat mem_cat /= in_cons in_nil !orb_false_r.
+        assert ((f ep) == (f eq) = false) as ->.
+        { apply /eqP => FPQ.
+          contradict Hneq.
+          apply F; trivial.
+          all: by rewrite !in_set; apply /eqP; apply nesym. }
+        rewrite orb_false_r.
+        apply /mapP. move => [[k b] K /= KEQ].
+        specialize (HPQ' _ K). clear K.
+        assert (ep = k).
+        { apply F; trivial.
+          - rewrite !in_set. apply /eqP. by apply nesym.
+          - rewrite !in_set. apply /eqP => FK.
+            contradict NPQ. apply /negP/negPn.
+            rewrite -FK.
+            replace k with ((k, b).1) by trivial.
+            by apply (map_f (fun e => f e.1)). }
+        subst k. clear KEQ.
+        revert HPQ'. rewrite /pq mem_cat upath_rev_in => /orP[In | In].
+        - contradict uP. apply /negP/negPn.
+          replace ep with ((ep, b).1) by trivial.
+          by apply (map_f (fun e => f e.1)).
+        - contradict Qep. apply /negP/negPn.
+          replace ep with ((ep, ~~b).1) by trivial.
+          by apply map_f. }
+      set PPQ'Q := supath_cat DP.
+      assert (Nnil : upval PPQ'Q <> [::]) by by [].
+      clearbody PPQ'Q. revert PPQ'Q Nnil. rewrite SP SQ => PPQ'Q Nnil.
+      contradict Nnil.
+      by rewrite (A _ PPQ'Q).
+Qed.
+(* Proof:
+  By induction, we can assume P and Q differ on their first edges, respectively ep and eq.
+  We denote by p and q the rest of P and Q respectively.
+  With p and q, we get a path pq from the target of ep to the target of eq (this is the part where we need
+  the infectivity of f).
+  Remark that q does not contain ep. Otherwise, (eq ++ q) would go back to s, by following q until
+  reaching ep (ep being in q or not according to signs). This would yield a non-trivial cycle,
+  contradicting acyclicity.
+  Similarly, p does not contain eq.
+  Thus, the path pq does not contain ep nor eq, as it is contain in the walk p ++ q.
+  But then, ep ++ pq ++ eq give us a non-trivial cycle, a contradiction
+*)
+
+Lemma utree_unique_path {I : finType} (f : edge G -> option I) :
+  {in ~: f @^-1 None &, injective f} -> utree f -> forall (s t : G),
+  { p : Supath f s t & forall (q : Supath f s t), p = q}.
+Proof.
+  intros F [A C] s t.
+  revert C => /(_ s t)/sigW[P _].
+  exists P.
+  by apply uacyclic_unique_path.
+Qed.
+
+(* Function to define a partition of the vertices of a tree: given a vertex v,
+   we partitione the tree into v itself, and a class for each edge of v,
+   containing vertices accessible from this edge *)
+Definition utree_part {I : finType} (f : edge G -> option I)
+  (F : {in ~: f @^-1 None &, injective f}) (T : utree f) (v : G) (x : G) : option (edge G) :=
+  match utree_unique_path F T v x with
+  | existT {| upval := [::] ; upvalK := _|} _        => None   (* class of v *)
+  | existT {| upval := (e, _) :: _ ; upvalK := _|} _ => Some e (* a class for each edge of v *)
+  end.
+
+(* In a tree, for any vertex v, we can partition the graph according to the edges of v *)
+Lemma tree_partition {I : finType} (f : edge G -> option I)
+  (F : {in ~: f @^-1 None &, injective f}) (T : utree f) (v : G) :
+  partition (preim_partition (utree_part F T v) setT) setT.
+Proof. exact (preim_partitionP (utree_part F T v) setT). Qed. (* TODO notation? *)
+
+Lemma inside_utree_part (S : {set G}) {I : finType} (f : edge G -> option I)
+  (F : {in ~: f @^-1 None &, injective f}) (T : utree f) (v : G) :
+  S \in (preim_partition (utree_part F T v) [set: G]) ->
+  forall a p (x : G) (X : x \in S),
+  supath f v x (a :: p) ->
+  forall e, e \in p -> e.1 \in edge_set S.
+Proof.
+  intros Sin a p.
+  induction p as [ | p ep IH] using last_ind; first by by [].
+  intros x X P e E.
+  rewrite -rcons_cons in P.
+  assert (P' := P).
+  rewrite supath_rcons in P. revert P => /andP[/andP[/andP[P /eqP-?] ?] ?]. subst x.
+  enough (TepS : usource ep \in S).
+  { specialize (IH _ TepS P).
+    revert E. rewrite in_rcons => /orP[/eqP-? | ]; last by apply IH.
+    subst e. rewrite /= in_set.
+    destruct ep as [? []]; splitb. }
+  clear IH E e.
+  apply (preim_partition_im_eq Sin X); trivial.
+  clear Sin X S.
+  unfold utree_part.
+  destruct (utree_unique_path F T v (usource ep)) as [[ps Ps] Us].
+  assert (ps = a :: p).
+  { specialize (Us {| upvalK := P |}). by inversion Us. }
+  subst ps. clear Us Ps .
+  destruct (utree_unique_path F T v (utarget ep)) as [[pt Pt] Ut].
+  assert (pt = rcons (a :: p) ep).
+  { specialize (Ut {| upvalK := P' |}). by inversion Ut. }
+  subst pt. clear Ut Pt P'.
+  reflexivity.
+Qed.
+
+Lemma uconnected_utree_part_in (S : {set G})
+  {I : finType} (f : edge G -> option I)
+  (F : {in ~: f @^-1 None &, injective f}) (T : utree f) (v : G) :
+  S \in (preim_partition (utree_part F T v) [set: G]) ->
+  forall x y, x \in S -> y \in S ->
+  forall e, e \in upval (projT1 (utree_unique_path F T x y)) -> e.1 \in edge_set S.
+(* Sketch of the proof :
+   We have a path from v to x and one from v to y.
+   Their concatenation, after reversing the first path and simplification,
+   yields the unique path from x to y.
+   This is a subpath of the previous two paths, without their
+   first edges (the one involving v).
+   These subpaths are included in S by Lemma inside_utree_part. *)
+Proof.
+  intros Sin x y X Y.
+  destruct (utree_unique_path F T x y) as [P Pu]. simpl.
+  assert (XY := preim_partition_in_eq Sin X Y).
+  unfold utree_part in XY.
+  destruct (utree_unique_path F T v x) as [[px Px] _].
+  destruct (utree_unique_path F T v y) as [[py Py] _].
+  destruct px as [ | (ex, box) px], py as [ | (ey, boy) py]; try by [].
+  { revert Px Py => /supath_of_nilP-? /supath_of_nilP-?. subst x y.
+    specialize (Pu (supath_nil _ v)). by subst P. }
+  inversion XY. subst ey. clear XY.
+  assert (PxS := inside_utree_part Sin X Px).
+  assert (PyS := inside_utree_part Sin Y Py).
+  rewrite !supath_cons in Px, Py.
+  revert Px => /andP[/andP[/andP[Px /eqP-Usex] _] /eqP-FexN]. simpl in FexN.
+  revert Py => /andP[/andP[/andP[Py /eqP-Usey] _] _].
+  assert (box = boy).
+  { clear P Pu px Px PxS py Py PyS x X y Y Sin F.
+    destruct T as [A _].
+    destruct (eq_comparable box boy) as [ | B]; trivial.
+    apply nesym in FexN. assert (F := uacyclic_loop A FexN). contradict F.
+    subst v. by destruct box, boy. }
+  subst boy. clear Usey Usex FexN.
+  apply supath_revK in Px. revert Px => /andP[/andP[Wx _] Nx].
+  revert Py => /andP[/andP[Wy _] Ny].
+  assert (Nxy : None \notin [seq f _e.1 | _e <- upath_rev px ++ py]).
+  { by rewrite map_cat mem_cat negb_orb Nx Ny. }
+  destruct (uconnected_simpl F (uwalk_cat Wx Wy) Nxy) as [Pxy Exy].
+  specialize (Pu Pxy). subst Pxy.
+  clear Nx Ny Nxy Wx Wy ex box X Y Sin T F.
+  intros (e, b) E.
+  revert Exy => /(_ _ E) {E}. rewrite mem_cat upath_rev_in => /orP[E | E].
+  - exact (PxS _ E).
+  - exact (PyS _ E).
+Qed.
+
+(* The patition of a tree yields connected components *)
+Lemma uconnected_utree_part (S : {set G})
+  {I J : finType} (f : edge G -> option I) (f' : edge (induced S) -> option J)
+  (F : {in ~: f @^-1 None &, injective f}) (T : utree f) (v : G) :
+  (forall e (E : e \in edge_set S), None <> f e -> None <> f' (Sub e E : edge (induced S))) ->
+  (forall e a (E : e \in edge_set S) (A : a \in edge_set S),
+    f' (Sub e E) = f' (Sub a A) -> f e = f a) ->
+  S \in (preim_partition (utree_part F T v) [set: G]) -> uconnected f'.
+Proof.
+  intros F0 F1 Sin [x X] [y Y].
+  destruct (supath_to_induced F0 F1 (uconnected_utree_part_in Sin X Y) X Y) as [Q _].
+  by exists Q.
+Qed.
+(* TODO voir ce qui tient avec cette définition de f', plus générale *)
+
+Lemma utree_part_None {I : finType} (f : edge G -> option I)
+  (F : {in ~: f @^-1 None &, injective f}) (T : utree f) (v x : G) :
+  utree_part F T v x = None -> x = v.
+Proof.
+  unfold utree_part.
+  destruct (utree_unique_path F T v x) as [[[ | (e, b) p] P] _]; last by [].
+  revert P. rewrite /supath /=. introb.
+Qed.
+
+Lemma utree_part_v_v {I : finType} (f : edge G -> option I)
+  (F : {in ~: f @^-1 None &, injective f}) (T : utree f) (v : G) :
+  utree_part F T v v = None.
+Proof.
+  unfold utree_part. destruct (utree_unique_path F T v v) as [P Pu].
+  specialize (Pu (supath_nil _ v)). by subst P.
+Qed.
+
+Lemma utree_part_v {I : finType} (f : edge G -> option I)
+  (F : {in ~: f @^-1 None &, injective f}) (T : utree f) (v : G) :
+  pblock (preim_partition (utree_part F T v) [set: G]) v = [set v].
+Proof.
+  assert (Spart := preim_partitionP (utree_part F T v) [set: G]).
+  revert Spart => /andP[/eqP-Cov /andP[Triv _]].
+  apply /setP => y.
+  rewrite in_set -eq_pblock // ?Cov // preim_partition_pblock_eq //.
+  destruct (eq_comparable y v) as [? | Y].
+  { subst y. by rewrite !eq_refl. }
+  transitivity false; last by (symmetry; apply /eqP).
+  rewrite utree_part_v_v.
+  destruct (utree_part F T v y) eqn:H; first by [].
+  contradict Y. by apply (utree_part_None H).
+Qed.
+
+End Tree.
