README.md
@@ -1,6 +1,6 @@
 # MLL Proof nets for Yalla
 
-Formalization of lieanr logic proof-nets for multiplicative linear logic in the spirit of the [Yalla library](https://perso.ens-lyon.fr/olivier.laurent/yalla/).
+Formalization of linear logic proof-nets for multiplicative linear logic in the spirit of the [Yalla library](https://perso.ens-lyon.fr/olivier.laurent/yalla/).
 
 Requires:
 - [OLlibs](https://github.com/olaure01/ollibs) (add-ons for the standard library): [see installation instructions](https://github.com/olaure01/ollibs/blob/master/README.md).
